---
title: "Lecture Proofs"
author: "Prof. Dr. Dominik Liebl" 
date: ""
output:
  pdf_document:
    includes:
      in_header: "preamble.tex"
---

```{r setup, include=FALSE}
knitr::opts_chunk$set(echo = TRUE)
```


# Review of Probability and Statistics

**Theorem:** For any events $A$ and $B$, we have that 
$$P(A \cup B)=P(A)+P(B)-P(A B)$$

**PROOF.** Write $A \cup B=\left(A B^{c}\right) \cup(A B) \cup\left(A^{c} B\right)$ and note that these events are disjoint. Hence, making repeated use of the fact that $P$ is additive for disjoint events, we see that
$$
\begin{aligned}
P(A \cup B) &=P\left(\left(A B^{r}\right) \cup(A B) \cup\left(A^{c} B\right)\right) \\
&=P\left(A B^{c}\right)+P(A B)+P\left(A^{c} B\right) \\
&=P\left(A B^{c}\right)+P(A B)+P\left(A^{c} B\right)+\Big(P(A B)-P(A B)\Big) \\
&=P\Big(\left(A B^{r}\right) \cup(A B)\Big)+P\Big(\left(A^{c} B\right) \cup(A B)\Big)-P(A B) \\
&=P(A)+P(B)-P(A B)
\end{aligned}
$$
qed

